fix notes

dialectica/ListT.v
@@ -7,24 +7,21 @@ Set Implicit Arguments.
 (** We use Mersenne induction to ensure that even if T may not be positive, that
     does not impede the writing of such a type. *)
 
-Inductive PlistT R (T : Type -> Type) A :=
-| NodeT : forall S, (S -> R + PnodeT R T A) -> T S -> PlistT R T A
+Inductive listT (T : Type -> Type) A :=
+| NodeT : forall S, (S -> nodeT T A) -> T S -> listT T A
 
-with PnodeT R (T : Type -> Type) A :=
-| Nil : PnodeT R T A
-| Cons : A -> PlistT R T A -> PnodeT R T A.
+with nodeT (T : Type -> Type) A :=
+| Nil : nodeT T A
+| Cons : A -> listT T A -> nodeT T A.
 
-Definition listT T A := PlistT False T A.
-Definition nodeT T A := PnodeT False T A.
-
-Arguments Nil [_ _ _].
+Arguments Nil [_ _].
 
 Fixpoint map {T A B} (f : A -> B) (l : listT T A) : listT T B
 with map_node {T A B} (f : A -> B) (n : nodeT T A) : nodeT T B.
 Proof.
 + destruct l as [S k n]; exists S.
-  - intros s; destruct (k s) as [[]|N].
-    right; apply (map_node _ A B f N).
+  - intros s.
+    apply (map_node T A B f (k s)).
   - exact n.
 + destruct n as [|x l].
   - apply Nil.
@@ -57,14 +54,34 @@ with fold_right_node {A B} (f : B -> A -> T A) (accu : T A) (n : nodeT T B) : T 
 Proof.
 + destruct l as [S k s].
   apply (@bind S); [clear s|exact s].
-  intros s; destruct (k s) as [[]|n].
-  apply (fold_right_node _ _ f accu n).
+  intros s; apply (fold_right_node _ _ f accu (k s)).
 + destruct n as [|x l].
   - exact accu.
   - pose (ans := fold_right _ _ f accu l).
     refine (bind _ ans); clear ans accu; intros accu.
     apply (f x accu).
 Defined.
+
+(* Definition collapse {A} (m : T (listT T A)) : listT T A.
+Proof.
+exists (T unit).
+exists (nodeT T A); [intros n; exact n|].
+refine (bind _ m).
+intros [S k s].
+refine (bind _ s); clear s; intros s.
+apply lift, (k s).
+Defined. *)
+
+Fixpoint app {A} (l1 l2 : listT T A) {struct l1} : listT T A
+with app_node {A} (n1 : nodeT T A) (l2 : listT T A) {struct n1} : listT T A.
+Proof.
++ destruct l1 as [S k s].
+  
+  apply app_node.
+  apply (app_node _ (k s) l2).
++ destruct n1 as [|x l1].
+  
+
 
 (* Fixpoint fold_right {A B} (f : B -> A -> T A) (accu : T A) (l : listT R T B) : T (R + A)
 with fold_right_node {A B} (f : B -> A -> T A) (accu : T A) (n : nodeT R T B) : T (R + A).
@@ -82,19 +99,21 @@ Proof.
     { refine (bind _ (f x accu)); intros ans; apply lift, inr, ans. }
 Defined.*)
 
-(* Definition collapse {A} (m : T (listT T A)) : listT T A.
+(*Definition collapse {A} (m : T (listT T A)) : listT T A.
 Proof.
-exists (nodeT T A); [exact inr|].
+exists (PnodeT False T A); [exact inr|].
 refine (bind _ m).
 intros [S k s].
 refine (bind _ s); clear s; intros s.
 destruct (k s) as [[]|n]; apply lift, n.
-Defined.*)
+Defined. *)
 
 Definition nil {A} : (listT T A) := NodeT (fun _ => inr Nil) (lift tt).
 Definition cons {A} (x : A) (l : listT T A) := NodeT (fun _ => inr (Cons x l)) (lift tt).
 
-(* Lemma toto : forall A B (f : A -> B) l,
-  map f l ≅ fold_right (fun x accu => lift (cons (f x) accu)) (lift nil) l.
- *)
+Lemma toto : forall A B (f : A -> B) l,
+  lift (map f l) ≅ fold_right (fun x accu => lift (cons (f x) accu)) (lift nil) l.
+Proof.
+intros A B f [S k s] Hext; simpl.
+
 End Ops.
